all new files added

SIL-Parallel/SIL_Single_Step_Sound.thy
@@ -10,29 +10,27 @@ lemma sil_single_step_sound:
   "\<turnstile> \<langle>P\<rangle>c \<leadsto> c'\<langle>R\<rangle>  \<Longrightarrow>  \<Turnstile> \<langle>P\<rangle>c \<leadsto> c'\<langle>R\<rangle>"
   unfolding SIL_Single_Step_Valid_def
   apply (induction rule:SIL_Single_Step.induct; fastforce?)
-         apply (case_tac R)
-         apply (clarsimp)
+            apply (case_tac R)
+            apply (clarsimp)
+            apply fastforce
+           apply fastforce
+          apply (case_tac Q)
+       apply clarsimp
+      apply fastforce
+            apply (case_tac Q)
+            apply clarsimp
+          apply fastforce
+         apply (case_tac Q)
+         apply clarsimp
          apply fastforce
-    apply fastforce
-   apply (case_tac Q)
-  apply clarsimp
-   apply fastforce
-  apply (case_tac Q)
-  apply clarsimp
+        apply (case_tac R)
+        apply clarsimp
+        apply fastforce
+       apply clarsimp
+       apply fastforce
+      apply (case_tac R)
+      apply clarsimp
+      apply fastforce
   by fastforce
 
-definition wp_single :: "com \<Rightarrow> com \<Rightarrow> post \<Rightarrow> assn" where
-  "wp_single c1 c2 R = (\<lambda>s. case R of
-      OK Q \<Rightarrow> (\<exists>s'. (c1,sOK s) \<rightarrow> (c2,sOK s') \<and> Q s')
-    | ER Q \<Rightarrow> (\<exists>s'. (c1,sOK s) \<rightarrow> (c2,sER s') \<and> Q s'))"
-
-
-lemma wp_single_ABORT: "wp_single ABORT SKIP R = (case R of
-      OK Q \<Rightarrow> (\<lambda>s. False)
-    | ER Q \<Rightarrow> Q)" 
-  apply (case_tac R)
-   apply clarsimp
-  unfolding wp_single_def apply fastforce
-  apply clarsimp
-  unfolding wp_single_def apply fastforce
-  done
+end
