SIL-Parallel/SIL_Single_Step_Complete.thy
@@ -1,0 +1,102 @@
+subsection \<open>Soundness and Completeness\<close>
+
+theory SIL_Single_Step_Complete
+imports SIL_Single_Step SIL_Single_Step_WP SIL_Single_Step_Sound
+begin
+
+subsubsection "Soundness"
+
+lemma seq_wp_single_is_pre:
+  assumes "\<turnstile> \<langle>wp_single c\<^sub>1 c' Q\<rangle> c\<^sub>1 \<leadsto> c' \<langle>Q\<rangle>"
+  and " \<turnstile> \<langle>wp_single c\<^sub>2 c' Q\<rangle> c\<^sub>2 \<leadsto> c' \<langle>Q\<rangle>"
+shows "\<turnstile> \<langle>wp_single (c\<^sub>1;;c\<^sub>2) c' Q\<rangle> c\<^sub>1;;c\<^sub>2 \<leadsto> c' \<langle>Q\<rangle>"
+
+proof(cases "c\<^sub>1 = SKIP")
+  case True
+  obtain Q' where  assn: "Q' = post_assn Q"
+    by auto
+  have h0: "\<turnstile> \<langle>\<lambda>s. Q' s \<and> c\<^sub>2 = c'\<rangle> c\<^sub>1;; c\<^sub>2 \<leadsto> c' \<langle>OK Q'\<rangle>"
+    by (metis sSubstituteCom sSeqSkip True)
+  have h1: "\<forall>s. wp_single (c\<^sub>1;;c\<^sub>2) c' (OK Q') s \<longrightarrow>  Q' s \<and> c\<^sub>2 = c'"
+    unfolding wp_single_def
+    using True by auto
+  have h2: " \<turnstile> \<langle>wp_single (c\<^sub>1;;c\<^sub>2) c' (OK Q')\<rangle> c\<^sub>1;; c\<^sub>2 \<leadsto> c' \<langle>OK Q'\<rangle>"
+    unfolding wp_single_def
+    using wp_single_Seq_OK h0 h1 sConseqOK wp_single_def
+    by auto
+ have h3: "\<forall>s. wp_single (c\<^sub>1;;c\<^sub>2) c' (ER Q') s \<longrightarrow>  False"
+    unfolding wp_single_def
+    using True by auto
+  have h4: "\<turnstile> \<langle>wp_single (c\<^sub>1;;c\<^sub>2) c' (ER Q')\<rangle> c\<^sub>1;; c\<^sub>2 \<leadsto> c' \<langle>ER Q'\<rangle>"
+    using h3 sFalsePre by presburger
+  then show ?thesis by (metis assn h2 h4 post_assn.elims)
+next
+  case False
+  then show ?thesis sorry
+qed
+ 
+
+
+
+lemma wp_single_is_pre: 
+  "\<turnstile> \<langle>wp_single c c' Q\<rangle> c \<leadsto> c' \<langle>Q\<rangle>"
+proof(induction c arbitrary: Q)
+  case SKIP
+  then show ?case 
+    apply (cases Q)
+    apply (metis wp_single_SKIP_OK sFalsePre strengthen_pre)
+    by (metis wp_single_SKIP_ER sFalsePre strengthen_pre)
+next
+  case ABORT
+  then show ?case
+    apply (cases Q)
+    apply (metis wp_single_ABORT_OK sFalsePre strengthen_pre)
+    by (metis sFalsePre strengthen_pre wp_single_ABORT_ER sAbort)
+next
+  case (Assign x1 x2)
+  then show ?case 
+    apply (cases Q)
+    apply (metis Assign' sFalsePre strengthen_pre wp_single_Assign_OK)
+    by (metis wp_single_Assign_ER sFalsePre strengthen_pre)
+next
+  case (AssignND x1 x2)
+  then show ?case
+    apply(cases Q)
+    using  wp_single_AssignND_OK
+    apply (smt (verit, best) sAssignNDEmpty sAssignNDOK sFalsePre strengthen_pre
+        wp_single_AssignND_Empty_OK)
+    by (metis wp_single_AssignND_ER sFalsePre strengthen_pre)
+next
+  case (Seq c1 c2)
+  then show ?case by (simp add: seq_wp_single_is_pre)
+next
+  case (If x1 c1 c2)
+  then show ?case
+    apply(cases Q)
+    using wp_single_If_OK sorry
+next
+  case (SelectND x)
+  then show ?case sorry
+next
+  case (While x1 c)
+  then show ?case sorry
+next
+  case (Par c1 c2)
+  then show ?case sorry
+qed
+
+
+lemma valid_imp_wp: "\<Turnstile> \<langle>P\<rangle> c \<leadsto> c'\<langle>Q\<rangle> \<Longrightarrow>  \<forall>s. P s \<longrightarrow> wp_single c c' Q s"
+  unfolding wp_single_def SIL_Single_Step_Valid_def
+  apply(cases Q)
+by fastforce+
+
+lemma sil_complete: 
+  "\<Turnstile> \<langle>P\<rangle> c \<leadsto> c'\<langle>Q\<rangle> \<Longrightarrow> \<turnstile> \<langle>P\<rangle> c \<leadsto> c'\<langle>Q\<rangle>"
+  apply (rule strengthen_pre[where P="wp_single c c' Q"])
+  apply (metis valid_imp_wp)
+by (metis wp_is_pre)
+
+corollary sil_sound_complete: 
+  "\<turnstile> \<langle>P\<rangle> c \<leadsto> c'\<langle>Q\<rangle> \<longleftrightarrow> \<Turnstile> \<langle>P\<rangle> c \<leadsto> c'\<langle>Q\<rangle>"
+by(fastforce simp: sil_single_step_sound sil_complete)
